theories/Generalization/GeneralizeLtsOutputs.v
@@ -20,12 +20,12 @@
    SOFTWARE.
 *)
 
-From Coq Require ssreflect Setoid.
-From Coq.Unicode Require Import Utf8.
-From Coq.Lists Require Import List.
+From Stdlib Require ssreflect Setoid.
+From Stdlib.Unicode Require Import Utf8.
+From Stdlib.Lists Require Import List.
 Import ListNotations.
-From Coq.Program Require Import Wf Equality.
-From Coq.Wellfounded Require Import Inverse_Image.
+From Stdlib.Program Require Import Wf Equality.
+From Stdlib.Wellfounded Require Import Inverse_Image.
 
 From stdpp Require Import base countable list decidable finite gmap gmultiset.
 From Must Require Import gLts InputOutputActions OldTransitionSystems Subset_Act
@@ -523,7 +523,7 @@ Proof.
 Qed.
 
 Lemma fw_does_all_input
-  `{@gLtsObaFW Q (ExtAct A) (@gLabel_nb A L) LtsQ LtsEqQ LtsObaQ} :
+  `{@gLtsObaFW Q (ExtAct A) (@gLabel_nb A L) LtsEqQ LtsObaQ} :
    forall (q' : Q) μ, ¬ is_output μ -> μ ∈ actions_of q'.
 Proof.
   intros q' μ not_nb. destruct μ as [ (* Input *) a | (* Output *) a].
